AwsEncryptionSDK/dafny/AwsEncryptionSdk/test/TestReproducedEncContext.dfy
@@ -1,0 +1,173 @@
+// Copyright Amazon.com Inc. or its affiliates. All Rights Reserved.
+// SPDX-License-Identifier: Apache-2.0
+
+include "../src/Index.dfy"
+
+include "Fixtures.dfy"
+
+module TestReproducedEncryptionContext {
+    import Types = AwsCryptographyEncryptionSdkTypes
+    import mplTypes = AwsCryptographyMaterialProvidersTypes
+    import MaterialProviders
+    import EncryptionSdk
+    import opened Wrappers
+
+    import Fixtures
+    
+    method {:test} TestEncryptionContextOnDecrypt()
+    {
+        var kmsKey :=  Fixtures.keyArn;
+        // The string "asdf" as bytes
+        var asdf := [ 97, 115, 100, 102 ];
+
+        var defaultConfig := EncryptionSdk.DefaultAwsEncryptionSdkConfig();
+        var esdk :- expect EncryptionSdk.ESDK(config := defaultConfig);
+        var mpl :- expect MaterialProviders.MaterialProviders();
+        var clientSupplier :- expect mpl.CreateDefaultClientSupplier(mplTypes.CreateDefaultClientSupplierInput);
+        var kmsClient :- expect clientSupplier.GetClient(mplTypes.GetClientInput(region := "us-west-2"));
+
+        var kmsKeyring :- expect mpl.CreateAwsKmsKeyring(
+            mplTypes.CreateAwsKmsKeyringInput(
+                kmsKeyId := kmsKey,
+                kmsClient := kmsClient,
+                grantTokens := None
+            )
+        );
+        
+        var encryptionContext := Fixtures.SmallEncryptionContext(Fixtures.SmallEncryptionContextVariation.AB);
+        
+        var encryptOutput := esdk.Encrypt(Types.EncryptInput(
+            plaintext := asdf,
+            encryptionContext := Some(encryptionContext), 
+            materialsManager := None,
+            keyring := Some(kmsKeyring),
+            algorithmSuiteId := None,
+            frameLength := None
+        ));
+        
+        expect encryptOutput.Success?;
+        var esdkCiphertext := encryptOutput.value.ciphertext;
+
+        var decryptOutput := esdk.Decrypt(Types.DecryptInput(
+            ciphertext := esdkCiphertext,
+            materialsManager := None,
+            keyring := Some(kmsKeyring),
+            encryptionContext := Some(encryptionContext)
+        ));
+
+        expect decryptOutput.Success?;
+        var cycledPlaintext := decryptOutput.value.plaintext;
+
+        expect cycledPlaintext == asdf;
+    }
+
+    method {:test} TestEncryptionContextOnDecryptFailure()
+    {
+        var kmsKey :=  Fixtures.keyArn;
+        // The string "asdf" as bytes
+        var asdf := [ 97, 115, 100, 102 ];
+
+        var defaultConfig := EncryptionSdk.DefaultAwsEncryptionSdkConfig();
+        var esdk :- expect EncryptionSdk.ESDK(config := defaultConfig);
+        var mpl :- expect MaterialProviders.MaterialProviders();
+        var clientSupplier :- expect mpl.CreateDefaultClientSupplier(mplTypes.CreateDefaultClientSupplierInput);
+        var kmsClient :- expect clientSupplier.GetClient(mplTypes.GetClientInput(region := "us-west-2"));
+        
+        var kmsKeyring :- expect mpl.CreateAwsKmsKeyring(
+            mplTypes.CreateAwsKmsKeyringInput(
+                kmsKeyId := kmsKey,
+                kmsClient := kmsClient,
+                grantTokens := None
+            )
+        );
+        
+        var encryptionContext := Fixtures.SmallEncryptionContext(Fixtures.SmallEncryptionContextVariation.A);
+        var incorrectReproducedEncryptionContext := Fixtures.SmallEncryptionContext(Fixtures.SmallEncryptionContextVariation.AB);
+        
+        var encryptOutput := esdk.Encrypt(Types.EncryptInput(
+            plaintext := asdf,
+            encryptionContext := Some(encryptionContext), 
+            materialsManager := None,
+            keyring := Some(kmsKeyring),
+            algorithmSuiteId := None,
+            frameLength := None
+        ));
+        
+        expect encryptOutput.Success?;
+        var esdkCiphertext := encryptOutput.value.ciphertext;
+
+        var decryptOutput := esdk.Decrypt(Types.DecryptInput(
+            ciphertext := esdkCiphertext,
+            materialsManager := None,
+            keyring := Some(kmsKeyring),
+            encryptionContext := Some(incorrectReproducedEncryptionContext)
+        ));
+        
+        // We expect to fail because we pass more encryption context than was used on encrypt
+        expect decryptOutput.Failure?;
+    }
+
+    method {:test} TestMismatchedEncryptionContextOnDecrypt()
+    {
+        // The string "asdf" as bytes
+        var asdf := [ 97, 115, 100, 102 ];
+        
+        var namespace, name := Fixtures.NamespaceAndName(0);
+        var defaultConfig := EncryptionSdk.DefaultAwsEncryptionSdkConfig();
+        var esdk :- expect EncryptionSdk.ESDK(config := defaultConfig);
+        var mpl :- expect MaterialProviders.MaterialProviders();
+        var rawAESKeyring :- expect mpl.CreateRawAesKeyring(mplTypes.CreateRawAesKeyringInput(
+                                                            keyNamespace := namespace,
+                                                            keyName := name,
+                                                            wrappingKey := seq(32, i => 0),
+                                                            wrappingAlg := mplTypes.ALG_AES256_GCM_IV12_TAG16
+                                                            ));
+        
+        var encryptionContext := Fixtures.SmallEncryptionContext(Fixtures.SmallEncryptionContextVariation.A);
+        var mismatchedEncryptionContext := Fixtures.SmallMismatchedEncryptionContex(Fixtures.SmallEncryptionContextVariation.A);
+        
+        var encryptOutput := esdk.Encrypt(Types.EncryptInput(
+            plaintext := asdf,
+            encryptionContext := Some(encryptionContext), 
+            materialsManager := None,
+            keyring := Some(rawAESKeyring),
+            algorithmSuiteId := None,
+            frameLength := None
+        ));
+        
+        expect encryptOutput.Success?;
+        var esdkCiphertext := encryptOutput.value.ciphertext;
+
+        var decryptOutput := esdk.Decrypt(Types.DecryptInput(
+            ciphertext := esdkCiphertext,
+            materialsManager := None,
+            keyring := Some(rawAESKeyring),
+            encryptionContext := Some(mismatchedEncryptionContext)
+        ));
+        
+        // We expect to fail because although the same key is present on the ec
+        // their value is different. 
+        expect decryptOutput.Failure?;
+        
+        // test that if we supply the right ec we will succeed
+        decryptOutput := esdk.Decrypt(Types.DecryptInput(
+                    ciphertext := esdkCiphertext,
+                    materialsManager := None,
+                    keyring := Some(rawAESKeyring),
+                    encryptionContext := Some(encryptionContext)
+                ));
+        
+        expect decryptOutput.Success?;
+
+        // Since we store all encryption context we MST succeed if no encryption context is
+        // supplied on decrypt
+        decryptOutput := esdk.Decrypt(Types.DecryptInput(
+                    ciphertext := esdkCiphertext,
+                    materialsManager := None,
+                    keyring := Some(rawAESKeyring),
+                    encryptionContext := None 
+                ));
+        
+        expect decryptOutput.Success?;
+    }
+}
