AwsEncryptionSDK/dafny/AwsEncryptionSdk/test/TestRequiredEncryptionContext.dfy
@@ -1,0 +1,1152 @@
+// Copyright Amazon.com Inc. or its affiliates. All Rights Reserved.
+// SPDX-License-Identifier: Apache-2.0
+
+include "../src/Index.dfy"
+
+include "Fixtures.dfy"
+
+module TestRequiredEncryptionContext {
+    import Types = AwsCryptographyEncryptionSdkTypes
+    import mplTypes = AwsCryptographyMaterialProvidersTypes
+    import primitivesTypes = AwsCryptographyPrimitivesTypes
+    import KeyStoreTypes = AwsCryptographyKeyStoreTypes
+    import MaterialProviders
+    import KeyStore
+    import ComAmazonawsKmsTypes
+    import KMS = Com.Amazonaws.Kms
+    import DDB = Com.Amazonaws.Dynamodb
+    import DDBTypes = ComAmazonawsDynamodbTypes
+    import EncryptionSdk
+    import opened Wrappers
+    import UTF8
+
+    import Fixtures
+    
+    // THIS IS A TESTING RESOURCE DO NOT USE IN A PRODUCTION ENVIRONMENT
+    const keyArn := Fixtures.keyArn
+    const hierarchyKeyArn := Fixtures.hierarchyKeyArn;
+    const branchKeyStoreName: DDBTypes.TableName := Fixtures.branchKeyStoreName
+    const logicalKeyStoreName := branchKeyStoreName
+    // These tests require a keystore populated with these keys
+    const BRANCH_KEY_ID := Fixtures.branchKeyId
+    
+    method {:test} TestReprEncryptionContextWithSameECHappyCase()
+    {
+        // The string "asdf" as bytes
+        var asdf := [ 97, 115, 100, 102 ];
+        
+        var defaultConfig := EncryptionSdk.DefaultAwsEncryptionSdkConfig();
+        var esdk :- expect EncryptionSdk.ESDK(config := defaultConfig);
+        var mpl :- expect MaterialProviders.MaterialProviders();
+
+        // get keyrings
+        var rsaKeyring := GetRsaKeyring();
+        var kmsKeyring := GetKmsKeyring();
+        var aesKeyring := GetAesKeyring();
+        var hKeyring := GetHierarchicalKeyring();
+        
+        var multiKeyring :- expect mpl.CreateMultiKeyring(mplTypes.CreateMultiKeyringInput(
+                                                            generator := Some(aesKeyring),
+                                                            childKeyrings := [rsaKeyring, kmsKeyring, hKeyring]
+                                                        ));
+
+        // HAPPY CASE 1
+        // Test supply same encryption context on encrypt and decrypt NO filtering
+        var encryptionContext := Fixtures.SmallEncryptionContext(Fixtures.SmallEncryptionContextVariation.AB);
+
+        var encryptOutput := esdk.Encrypt(Types.EncryptInput(
+            plaintext := asdf,
+            encryptionContext := Some(encryptionContext), 
+            materialsManager := None,
+            keyring := Some(multiKeyring),
+            algorithmSuiteId := None,
+            frameLength := None
+        ));
+        
+        expect encryptOutput.Success?;
+        var esdkCiphertext := encryptOutput.value.ciphertext;
+        
+        // Test RSA
+        var decryptOutput := esdk.Decrypt(Types.DecryptInput(
+            ciphertext := esdkCiphertext,
+            materialsManager := None,
+            keyring := Some(rsaKeyring),
+            encryptionContext := Some(encryptionContext)
+        ));
+        
+        expect decryptOutput.Success?;
+        var cycledPlaintext := decryptOutput.value.plaintext;
+        expect cycledPlaintext == asdf;
+        
+        // Test KMS
+        decryptOutput := esdk.Decrypt(Types.DecryptInput(
+            ciphertext := esdkCiphertext,
+            materialsManager := None,
+            keyring := Some(kmsKeyring),
+            encryptionContext := Some(encryptionContext)
+        ));
+        
+        expect decryptOutput.Success?;
+        cycledPlaintext := decryptOutput.value.plaintext;
+        expect cycledPlaintext == asdf;
+        
+        // Test AES
+        decryptOutput := esdk.Decrypt(Types.DecryptInput(
+            ciphertext := esdkCiphertext,
+            materialsManager := None,
+            keyring := Some(aesKeyring),
+            encryptionContext := Some(encryptionContext)
+        ));
+        
+        expect decryptOutput.Success?;
+        cycledPlaintext := decryptOutput.value.plaintext;
+        expect cycledPlaintext == asdf;
+        
+        // Test Hierarchy Keyring
+        decryptOutput := esdk.Decrypt(Types.DecryptInput(
+            ciphertext := esdkCiphertext,
+            materialsManager := None,
+            keyring := Some(hKeyring),
+            encryptionContext := Some(encryptionContext)
+        ));
+        
+        expect decryptOutput.Success?;
+        cycledPlaintext := decryptOutput.value.plaintext;
+        expect cycledPlaintext == asdf;
+    }
+
+    method {:test} TestRemoveOnEncryptAndSupplyOnDecryptHappyCase()
+    {
+        // The string "asdf" as bytes
+        var asdf := [ 97, 115, 100, 102 ];
+        
+        var defaultConfig := EncryptionSdk.DefaultAwsEncryptionSdkConfig();
+        var esdk :- expect EncryptionSdk.ESDK(config := defaultConfig);
+        var mpl :- expect MaterialProviders.MaterialProviders();
+
+        // get keyrings
+        var rsaKeyring := GetRsaKeyring();
+        var kmsKeyring := GetKmsKeyring();
+        var aesKeyring := GetAesKeyring();
+        var hKeyring := GetHierarchicalKeyring();
+
+        var multiKeyring :- expect mpl.CreateMultiKeyring(mplTypes.CreateMultiKeyringInput(
+                                                            generator := Some(aesKeyring),
+                                                            childKeyrings := [rsaKeyring, kmsKeyring, hKeyring]
+                                                        ));
+
+        // Happy Test Case 2
+        // On Encrypt we will only write one encryption context key value to the header
+        // we will then supply only what we didn't write wth no required ec cmm,
+        // This test case is checking that the default cmm is doing the correct filtering by using
+        var encryptionContext := Fixtures.SmallEncryptionContext(Fixtures.SmallEncryptionContextVariation.AB);
+        var reproducedEncryptionContext := Fixtures.SmallEncryptionContext(Fixtures.SmallEncryptionContextVariation.A);
+        // These keys mean that we will not write these on the message but are required for message authentication on decrypt.
+        var requiredEncryptionContextKeys := Fixtures.SmallEncryptionContextKeys(Fixtures.SmallEncryptionContextVariation.A);
+
+        // TEST RSA
+        var defaultCMM :- expect mpl.CreateDefaultCryptographicMaterialsManager(
+            mplTypes.CreateDefaultCryptographicMaterialsManagerInput(
+                keyring := multiKeyring
+            )
+        );
+
+        // Create Required EC CMM with the required EC Keys we want
+        var reqCMM :- expect mpl.CreateRequiredEncryptionContextCMM(
+            mplTypes.CreateRequiredEncryptionContextCMMInput(
+                underlyingCMM := Some(defaultCMM),
+                // At the moment reqCMM can only be created with a CMM, you cannot 
+                // create one by only passing in a keyring.
+                keyring := None,
+                requiredEncryptionContextKeys := requiredEncryptionContextKeys
+            )
+        );
+        
+        var encryptOutput := esdk.Encrypt(Types.EncryptInput(
+            plaintext := asdf,
+            encryptionContext := Some(encryptionContext), 
+            materialsManager := Some(reqCMM),
+            keyring := None,
+            algorithmSuiteId := None,
+            frameLength := None
+        ));
+        
+        expect encryptOutput.Success?;
+        var esdkCiphertext := encryptOutput.value.ciphertext;
+        
+        // Switch to only RSA keyring
+        var decryptOutput := esdk.Decrypt(Types.DecryptInput(
+            ciphertext := esdkCiphertext,
+            materialsManager := None,
+            keyring := Some(rsaKeyring),
+            encryptionContext := Some(reproducedEncryptionContext)
+        ));
+        
+        expect decryptOutput.Success?;
+        var cycledPlaintext := decryptOutput.value.plaintext;
+        expect cycledPlaintext == asdf;
+        
+        // Switch to only KMS keyring
+        decryptOutput := esdk.Decrypt(Types.DecryptInput(
+            ciphertext := esdkCiphertext,
+            materialsManager := None,
+            keyring := Some(kmsKeyring),
+            encryptionContext := Some(reproducedEncryptionContext)
+        ));
+        
+        expect decryptOutput.Success?;
+        cycledPlaintext := decryptOutput.value.plaintext;
+        expect cycledPlaintext == asdf;
+        
+        // Switch to only AES keyring
+        decryptOutput := esdk.Decrypt(Types.DecryptInput(
+            ciphertext := esdkCiphertext,
+            materialsManager := None,
+            keyring := Some(aesKeyring),
+            encryptionContext := Some(reproducedEncryptionContext)
+        ));
+        
+        expect decryptOutput.Success?;
+        cycledPlaintext := decryptOutput.value.plaintext;
+        expect cycledPlaintext == asdf;
+        
+        // Switch to only Hierarchical keyring
+        decryptOutput := esdk.Decrypt(Types.DecryptInput(
+            ciphertext := esdkCiphertext,
+            materialsManager := None,
+            keyring := Some(hKeyring),
+            encryptionContext := Some(reproducedEncryptionContext)
+        ));
+        
+        expect decryptOutput.Success?;
+        cycledPlaintext := decryptOutput.value.plaintext;
+        expect cycledPlaintext == asdf;
+
+    }
+
+    method {:test} TestRemoveOnEncryptRemoveAndSupplyOnDecryptHappyCase()
+    {
+        // The string "asdf" as bytes
+        var asdf := [ 97, 115, 100, 102 ];
+        
+        var defaultConfig := EncryptionSdk.DefaultAwsEncryptionSdkConfig();
+        var esdk :- expect EncryptionSdk.ESDK(config := defaultConfig);
+        var mpl :- expect MaterialProviders.MaterialProviders();
+
+        // get keyrings
+        var rsaKeyring := GetRsaKeyring();
+        var kmsKeyring := GetKmsKeyring();
+        var aesKeyring := GetAesKeyring();
+        var hKeyring := GetHierarchicalKeyring();
+
+        var multiKeyring :- expect mpl.CreateMultiKeyring(mplTypes.CreateMultiKeyringInput(
+                                                            generator := Some(aesKeyring),
+                                                            childKeyrings := [rsaKeyring, kmsKeyring, hKeyring]
+                                                        ));
+
+        // HAPPY CASE 3
+        // On Encrypt we will only write one encryption context key value to the header
+        // we will then supply only what we didn't write but included in the signature while we 
+        // are configured with the required encryption context cmm
+        var encryptionContext := Fixtures.SmallEncryptionContext(Fixtures.SmallEncryptionContextVariation.AB);
+        var reproducedEncryptionContext := Fixtures.SmallEncryptionContext(Fixtures.SmallEncryptionContextVariation.A);
+        // These keys mean that we will not write these on the message but are required for message authentication on decrypt.
+        var requiredEncryptionContextKeys := Fixtures.SmallEncryptionContextKeys(Fixtures.SmallEncryptionContextVariation.A);
+
+        // TEST RSA
+        var defaultCMM :- expect mpl.CreateDefaultCryptographicMaterialsManager(
+            mplTypes.CreateDefaultCryptographicMaterialsManagerInput(
+                keyring := multiKeyring
+            )
+        );
+
+        // Create Required EC CMM with the required EC Keys we want
+        var reqCMM :- expect mpl.CreateRequiredEncryptionContextCMM(
+            mplTypes.CreateRequiredEncryptionContextCMMInput(
+                underlyingCMM := Some(defaultCMM),
+                // At the moment reqCMM can only be created with a CMM, you cannot 
+                // create one by only passing in a keyring.
+                keyring := None,
+                requiredEncryptionContextKeys := requiredEncryptionContextKeys
+            )
+        );
+        
+        var encryptOutput := esdk.Encrypt(Types.EncryptInput(
+            plaintext := asdf,
+            encryptionContext := Some(encryptionContext), 
+            materialsManager := Some(reqCMM),
+            keyring := None,
+            algorithmSuiteId := None,
+            frameLength := None
+        ));
+        
+        expect encryptOutput.Success?;
+        var esdkCiphertext := encryptOutput.value.ciphertext;
+        
+        // Switch to only RSA keyring
+        defaultCMM :- expect mpl.CreateDefaultCryptographicMaterialsManager(
+            mplTypes.CreateDefaultCryptographicMaterialsManagerInput(
+                keyring := rsaKeyring
+            )
+        );
+
+        // Create Required EC CMM with the required EC Keys we want
+        reqCMM :- expect mpl.CreateRequiredEncryptionContextCMM(
+            mplTypes.CreateRequiredEncryptionContextCMMInput(
+                underlyingCMM := Some(defaultCMM),
+                // At the moment reqCMM can only be created with a CMM, you cannot 
+                // create one by only passing in a keyring.
+                keyring := None,
+                requiredEncryptionContextKeys := requiredEncryptionContextKeys
+            )
+        );
+        // Since we are passing in the correct reproduced encryption context this
+        // decrypt SHOULD succeed
+        var decryptOutput := esdk.Decrypt(Types.DecryptInput(
+            ciphertext := esdkCiphertext,
+            materialsManager := Some(reqCMM),
+            keyring := None,
+            encryptionContext := Some(reproducedEncryptionContext)
+        ));
+        
+        expect decryptOutput.Success?;
+        var cycledPlaintext := decryptOutput.value.plaintext;
+        expect cycledPlaintext == asdf;
+
+        // TEST KMS
+        // Switch to only KMS keyring
+        defaultCMM :- expect mpl.CreateDefaultCryptographicMaterialsManager(
+            mplTypes.CreateDefaultCryptographicMaterialsManagerInput(
+                keyring := kmsKeyring
+            )
+        );
+
+        // Create Required EC CMM with the required EC Keys we want
+        reqCMM :- expect mpl.CreateRequiredEncryptionContextCMM(
+            mplTypes.CreateRequiredEncryptionContextCMMInput(
+                underlyingCMM := Some(defaultCMM),
+                // At the moment reqCMM can only be created with a CMM, you cannot 
+                // create one by only passing in a keyring.
+                keyring := None,
+                requiredEncryptionContextKeys := requiredEncryptionContextKeys
+            )
+        );
+        // Since we are passing in the correct reproduced encryption context this
+        // decrypt SHOULD succeed
+        decryptOutput := esdk.Decrypt(Types.DecryptInput(
+            ciphertext := esdkCiphertext,
+            materialsManager := Some(reqCMM),
+            keyring := None,
+            encryptionContext := Some(reproducedEncryptionContext)
+        ));
+        
+        expect decryptOutput.Success?;
+        cycledPlaintext := decryptOutput.value.plaintext;
+        expect cycledPlaintext == asdf;
+        
+        // TEST AES
+        // switch to only aes
+        defaultCMM :- expect mpl.CreateDefaultCryptographicMaterialsManager(
+            mplTypes.CreateDefaultCryptographicMaterialsManagerInput(
+                keyring := aesKeyring 
+            )
+        );
+
+        // Create Required EC CMM with the required EC Keys we want
+        reqCMM :- expect mpl.CreateRequiredEncryptionContextCMM(
+            mplTypes.CreateRequiredEncryptionContextCMMInput(
+                underlyingCMM := Some(defaultCMM),
+                // At the moment reqCMM can only be created with a CMM, you cannot 
+                // create one by only passing in a keyring.
+                keyring := None,
+                requiredEncryptionContextKeys := requiredEncryptionContextKeys
+            )
+        );
+        // Since we are passing in the correct reproduced encryption context this
+        // decrypt SHOULD succeed
+        decryptOutput := esdk.Decrypt(Types.DecryptInput(
+            ciphertext := esdkCiphertext,
+            materialsManager := Some(reqCMM),
+            keyring := None,
+            encryptionContext := Some(reproducedEncryptionContext)
+        ));
+        
+        expect decryptOutput.Success?;
+        cycledPlaintext := decryptOutput.value.plaintext;
+        expect cycledPlaintext == asdf;
+
+        // TEST HIERARCHY
+        defaultCMM :- expect mpl.CreateDefaultCryptographicMaterialsManager(
+            mplTypes.CreateDefaultCryptographicMaterialsManagerInput(
+                keyring := hKeyring 
+            )
+        );
+
+        // Create Required EC CMM with the required EC Keys we want
+        reqCMM :- expect mpl.CreateRequiredEncryptionContextCMM(
+            mplTypes.CreateRequiredEncryptionContextCMMInput(
+                underlyingCMM := Some(defaultCMM),
+                // At the moment reqCMM can only be created with a CMM, you cannot 
+                // create one by only passing in a keyring.
+                keyring := None,
+                requiredEncryptionContextKeys := requiredEncryptionContextKeys
+            )
+        );
+        // Since we are passing in the correct reproduced encryption context this
+        // decrypt SHOULD succeed
+        decryptOutput := esdk.Decrypt(Types.DecryptInput(
+            ciphertext := esdkCiphertext,
+            materialsManager := Some(reqCMM),
+            keyring := None,
+            encryptionContext := Some(reproducedEncryptionContext)
+        ));
+        
+        expect decryptOutput.Success?;
+        cycledPlaintext := decryptOutput.value.plaintext;
+        expect cycledPlaintext == asdf;
+    }
+
+    method {:test} TestRemoveOnDecryptIsBackwardsCompatibleHappyCase()
+    {
+        // The string "asdf" as bytes
+        var asdf := [ 97, 115, 100, 102 ];
+        
+        var defaultConfig := EncryptionSdk.DefaultAwsEncryptionSdkConfig();
+        var esdk :- expect EncryptionSdk.ESDK(config := defaultConfig);
+        var mpl :- expect MaterialProviders.MaterialProviders();
+
+        // get keyrings
+        var rsaKeyring := GetRsaKeyring();
+        var kmsKeyring := GetKmsKeyring();
+        var aesKeyring := GetAesKeyring();
+        var hKeyring := GetHierarchicalKeyring();
+
+        var multiKeyring :- expect mpl.CreateMultiKeyring(mplTypes.CreateMultiKeyringInput(
+                                                            generator := Some(aesKeyring),
+                                                            childKeyrings := [rsaKeyring, kmsKeyring, hKeyring]
+                                                        ));
+
+        // HAPPY CASE 4
+        // On Encrypt we write all encryption context
+        // as if the message was encrypted before the feature existed.
+        // We will then have a required encryption context cmm
+        // that will require us to supply the encryption context on decrypt.
+        var encryptionContext := Fixtures.SmallEncryptionContext(Fixtures.SmallEncryptionContextVariation.AB);
+        var reproducedEncryptionContext := Fixtures.SmallEncryptionContext(Fixtures.SmallEncryptionContextVariation.A);
+        // These keys mean that we will not write these on the message but are required for message authentication on decrypt.
+        var requiredEncryptionContextKeys := Fixtures.SmallEncryptionContextKeys(Fixtures.SmallEncryptionContextVariation.A);
+
+        var defaultCMM :- expect mpl.CreateDefaultCryptographicMaterialsManager(
+            mplTypes.CreateDefaultCryptographicMaterialsManagerInput(
+                keyring := multiKeyring
+            )
+        );
+        
+        // All encryption context is stored in the message
+        var encryptOutput := esdk.Encrypt(Types.EncryptInput(
+            plaintext := asdf,
+            encryptionContext := Some(encryptionContext), 
+            materialsManager := Some(defaultCMM),
+            keyring := None,
+            algorithmSuiteId := None,
+            frameLength := None
+        ));
+        
+        expect encryptOutput.Success?;
+        var esdkCiphertext := encryptOutput.value.ciphertext;
+        
+        // Switch to only RSA keyring
+        defaultCMM :- expect mpl.CreateDefaultCryptographicMaterialsManager(
+            mplTypes.CreateDefaultCryptographicMaterialsManagerInput(
+                keyring := rsaKeyring
+            )
+        );
+
+        // Create Required EC CMM with the required EC Keys we want
+        var reqCMM :- expect mpl.CreateRequiredEncryptionContextCMM(
+            mplTypes.CreateRequiredEncryptionContextCMMInput(
+                underlyingCMM := Some(defaultCMM),
+                // At the moment reqCMM can only be created with a CMM, you cannot 
+                // create one by only passing in a keyring.
+                keyring := None,
+                requiredEncryptionContextKeys := requiredEncryptionContextKeys
+            )
+        );
+        // Since we are passing in the correct reproduced encryption context this
+        // decrypt SHOULD succeed
+        var decryptOutput := esdk.Decrypt(Types.DecryptInput(
+            ciphertext := esdkCiphertext,
+            materialsManager := Some(reqCMM),
+            keyring := None,
+            encryptionContext := Some(reproducedEncryptionContext)
+        ));
+        
+        expect decryptOutput.Success?;
+        var cycledPlaintext := decryptOutput.value.plaintext;
+        expect cycledPlaintext == asdf;
+
+        // TEST KMS
+        // Switch to only KMS keyring
+        defaultCMM :- expect mpl.CreateDefaultCryptographicMaterialsManager(
+            mplTypes.CreateDefaultCryptographicMaterialsManagerInput(
+                keyring := kmsKeyring
+            )
+        );
+
+        // Create Required EC CMM with the required EC Keys we want
+        reqCMM :- expect mpl.CreateRequiredEncryptionContextCMM(
+            mplTypes.CreateRequiredEncryptionContextCMMInput(
+                underlyingCMM := Some(defaultCMM),
+                // At the moment reqCMM can only be created with a CMM, you cannot 
+                // create one by only passing in a keyring.
+                keyring := None,
+                requiredEncryptionContextKeys := requiredEncryptionContextKeys
+            )
+        );
+        // Since we are passing in the correct reproduced encryption context this
+        // decrypt SHOULD succeed
+        decryptOutput := esdk.Decrypt(Types.DecryptInput(
+            ciphertext := esdkCiphertext,
+            materialsManager := Some(reqCMM),
+            keyring := None,
+            encryptionContext := Some(reproducedEncryptionContext)
+        ));
+        
+        expect decryptOutput.Success?;
+        cycledPlaintext := decryptOutput.value.plaintext;
+        expect cycledPlaintext == asdf;
+        
+        // TEST AES
+        // switch to only aes
+        defaultCMM :- expect mpl.CreateDefaultCryptographicMaterialsManager(
+            mplTypes.CreateDefaultCryptographicMaterialsManagerInput(
+                keyring := aesKeyring 
+            )
+        );
+
+        // Create Required EC CMM with the required EC Keys we want
+        reqCMM :- expect mpl.CreateRequiredEncryptionContextCMM(
+            mplTypes.CreateRequiredEncryptionContextCMMInput(
+                underlyingCMM := Some(defaultCMM),
+                // At the moment reqCMM can only be created with a CMM, you cannot 
+                // create one by only passing in a keyring.
+                keyring := None,
+                requiredEncryptionContextKeys := requiredEncryptionContextKeys
+            )
+        );
+        // Since we are passing in the correct reproduced encryption context this
+        // decrypt SHOULD succeed
+        decryptOutput := esdk.Decrypt(Types.DecryptInput(
+            ciphertext := esdkCiphertext,
+            materialsManager := Some(reqCMM),
+            keyring := None,
+            encryptionContext := Some(reproducedEncryptionContext)
+        ));
+        
+        expect decryptOutput.Success?;
+        cycledPlaintext := decryptOutput.value.plaintext;
+        expect cycledPlaintext == asdf;
+
+        // TEST HIERARCHY
+        defaultCMM :- expect mpl.CreateDefaultCryptographicMaterialsManager(
+            mplTypes.CreateDefaultCryptographicMaterialsManagerInput(
+                keyring := hKeyring 
+            )
+        );
+
+        // Create Required EC CMM with the required EC Keys we want
+        reqCMM :- expect mpl.CreateRequiredEncryptionContextCMM(
+            mplTypes.CreateRequiredEncryptionContextCMMInput(
+                underlyingCMM := Some(defaultCMM),
+                // At the moment reqCMM can only be created with a CMM, you cannot 
+                // create one by only passing in a keyring.
+                keyring := None,
+                requiredEncryptionContextKeys := requiredEncryptionContextKeys
+            )
+        );
+        // Since we are passing in the correct reproduced encryption context this
+        // decrypt SHOULD succeed
+        decryptOutput := esdk.Decrypt(Types.DecryptInput(
+            ciphertext := esdkCiphertext,
+            materialsManager := Some(reqCMM),
+            keyring := None,
+            encryptionContext := Some(reproducedEncryptionContext)
+        ));
+        
+        expect decryptOutput.Success?;
+        cycledPlaintext := decryptOutput.value.plaintext;
+        expect cycledPlaintext == asdf;
+    }
+
+    method {:test} TestDifferentECOnDecryptFailure()
+    {
+        // encrypt {a, b} => decrypt {b:c} => fail
+        // encrypt {a, b} => decrypt {d} => fail
+
+        // The string "asdf" as bytes
+        var asdf := [ 97, 115, 100, 102 ];
+        
+        var defaultConfig := EncryptionSdk.DefaultAwsEncryptionSdkConfig();
+        var esdk :- expect EncryptionSdk.ESDK(config := defaultConfig);
+        var mpl :- expect MaterialProviders.MaterialProviders();
+
+        // get keyrings
+        var rsaKeyring := GetRsaKeyring();
+        var kmsKeyring := GetKmsKeyring();
+        var aesKeyring := GetAesKeyring();
+        var hKeyring := GetHierarchicalKeyring();
+
+        var multiKeyring :- expect mpl.CreateMultiKeyring(mplTypes.CreateMultiKeyringInput(
+                                                            generator := Some(aesKeyring),
+                                                            childKeyrings := [rsaKeyring, kmsKeyring, hKeyring]
+                                                        ));
+
+        // FAILURE CASE 1
+        // Encrypt with and store all encryption context in header
+        // On Decrypt supply additional encryption context not stored in the header; this MUST fail
+        // On Decrypt supply mismatched encryption context key values; this MUST fail
+        var encryptionContext := Fixtures.SmallEncryptionContext(Fixtures.SmallEncryptionContextVariation.AB);
+        // Additional EC 
+        var reproducedAdditionalEncryptionContext := Fixtures.SmallEncryptionContext(Fixtures.SmallEncryptionContextVariation.C);
+        // Mismatched EncryptionContext
+        var reproducedMismatchedEncryptionContext := Fixtures.SmallMismatchedEncryptionContex(Fixtures.SmallEncryptionContextVariation.AB);
+        
+        var encryptOutput := esdk.Encrypt(Types.EncryptInput(
+            plaintext := asdf,
+            encryptionContext := Some(encryptionContext), 
+            materialsManager := None,
+            keyring := Some(multiKeyring),
+            algorithmSuiteId := None,
+            frameLength := None
+        ));
+        
+        expect encryptOutput.Success?;
+        var esdkCiphertext := encryptOutput.value.ciphertext;
+
+        // Test RSA Failures
+        var decryptOutput := esdk.Decrypt(Types.DecryptInput(
+            ciphertext := esdkCiphertext,
+            materialsManager := None,
+            keyring := Some(rsaKeyring),
+            encryptionContext := Some(reproducedAdditionalEncryptionContext)
+        ));
+        
+        expect decryptOutput.Failure?;
+        
+        decryptOutput := esdk.Decrypt(Types.DecryptInput(
+            ciphertext := esdkCiphertext,
+            materialsManager := None,
+            keyring := Some(rsaKeyring),
+            encryptionContext := Some(reproducedMismatchedEncryptionContext)
+        ));
+        
+        expect decryptOutput.Failure?;
+
+        // Test KMS Failures
+        decryptOutput := esdk.Decrypt(Types.DecryptInput(
+            ciphertext := esdkCiphertext,
+            materialsManager := None,
+            keyring := Some(kmsKeyring),
+            encryptionContext := Some(reproducedAdditionalEncryptionContext)
+        ));
+        
+        expect decryptOutput.Failure?;
+        
+        decryptOutput := esdk.Decrypt(Types.DecryptInput(
+            ciphertext := esdkCiphertext,
+            materialsManager := None,
+            keyring := Some(kmsKeyring),
+            encryptionContext := Some(reproducedMismatchedEncryptionContext)
+        ));
+        
+        expect decryptOutput.Failure?;
+
+        // Test AES Failures
+        decryptOutput := esdk.Decrypt(Types.DecryptInput(
+            ciphertext := esdkCiphertext,
+            materialsManager := None,
+            keyring := Some(aesKeyring),
+            encryptionContext := Some(reproducedAdditionalEncryptionContext)
+        ));
+        
+        expect decryptOutput.Failure?;
+        
+        decryptOutput := esdk.Decrypt(Types.DecryptInput(
+            ciphertext := esdkCiphertext,
+            materialsManager := None,
+            keyring := Some(aesKeyring),
+            encryptionContext := Some(reproducedMismatchedEncryptionContext)
+        ));
+        
+        expect decryptOutput.Failure?;
+
+        // Test Hierarchical Failures
+        decryptOutput := esdk.Decrypt(Types.DecryptInput(
+            ciphertext := esdkCiphertext,
+            materialsManager := None,
+            keyring := Some(hKeyring),
+            encryptionContext := Some(reproducedAdditionalEncryptionContext)
+        ));
+        
+        expect decryptOutput.Failure?;
+        
+        decryptOutput := esdk.Decrypt(Types.DecryptInput(
+            ciphertext := esdkCiphertext,
+            materialsManager := None,
+            keyring := Some(hKeyring),
+            encryptionContext := Some(reproducedMismatchedEncryptionContext)
+        ));
+        
+        expect decryptOutput.Failure?;
+    }
+
+    method {:test} TestRemoveECAndNotSupplyOnDecryptFailure()
+    {
+
+        // encrypt remove(a) RSA {a, b} => decrypt => fail
+        // encrypt remove(a) KMS {a, b} => decrypt => fail
+        // encrypt remove(a) AES {a, b} => decrypt => fail
+        // encrypt remove(a) Hie {a, b} => decrypt => fail
+        
+        // The string "asdf" as bytes
+        var asdf := [ 97, 115, 100, 102 ];
+        
+        var defaultConfig := EncryptionSdk.DefaultAwsEncryptionSdkConfig();
+        var esdk :- expect EncryptionSdk.ESDK(config := defaultConfig);
+        var mpl :- expect MaterialProviders.MaterialProviders();
+
+        // get keyrings
+        var rsaKeyring := GetRsaKeyring();
+        var kmsKeyring := GetKmsKeyring();
+        var aesKeyring := GetAesKeyring();
+        var hKeyring := GetHierarchicalKeyring();
+        
+        var multiKeyring :- expect mpl.CreateMultiKeyring(mplTypes.CreateMultiKeyringInput(
+                                                            generator := Some(aesKeyring),
+                                                            childKeyrings := [rsaKeyring, kmsKeyring, hKeyring]
+                                                        ));
+
+        // FAILURE CASE 2
+        // Encrypt will not store all Encryption Context, we will drop one entry but it will still get included in the 
+        // header signture.
+        // Decrypt will not supply any reproduced Encryption Context; this MUST fail.
+        var encryptionContext := Fixtures.SmallEncryptionContext(Fixtures.SmallEncryptionContextVariation.AB);
+        var requiredECKeys := Fixtures.SmallEncryptionContextKeys(Fixtures.SmallEncryptionContextVariation.A); 
+        
+        var defaultCMM :- expect mpl.CreateDefaultCryptographicMaterialsManager(
+            mplTypes.CreateDefaultCryptographicMaterialsManagerInput(
+                keyring := multiKeyring
+            )
+        );
+
+        // Create Required EC CMM with the required EC Keys we want
+        var reqCMM :- expect mpl.CreateRequiredEncryptionContextCMM(
+            mplTypes.CreateRequiredEncryptionContextCMMInput(
+                underlyingCMM := Some(defaultCMM),
+                // At the moment reqCMM can only be created with a CMM, you cannot 
+                // create one by only passing in a keyring.
+                keyring := None,
+                requiredEncryptionContextKeys := requiredECKeys
+            )
+        );
+
+        var encryptOutput := esdk.Encrypt(Types.EncryptInput(
+            plaintext := asdf,
+            encryptionContext := Some(encryptionContext), 
+            materialsManager := Some(reqCMM),
+            keyring := None,
+            algorithmSuiteId := None,
+            frameLength := None
+        ));
+        
+        expect encryptOutput.Success?;
+        var esdkCiphertext := encryptOutput.value.ciphertext;
+        
+        // Test RSA Failure
+        var decryptOutput := esdk.Decrypt(Types.DecryptInput(
+            ciphertext := esdkCiphertext,
+            materialsManager := None,
+            keyring := Some(rsaKeyring),
+            encryptionContext := None
+        ));
+        
+        expect decryptOutput.Failure?;
+
+        // Test KMS Failures
+        decryptOutput := esdk.Decrypt(Types.DecryptInput(
+            ciphertext := esdkCiphertext,
+            materialsManager := None,
+            keyring := Some(kmsKeyring),
+            encryptionContext := None
+        ));
+        
+        expect decryptOutput.Failure?;
+
+        // Test AES Failures
+        decryptOutput := esdk.Decrypt(Types.DecryptInput(
+            ciphertext := esdkCiphertext,
+            materialsManager := None,
+            keyring := Some(aesKeyring),
+            encryptionContext := None
+        ));
+        
+        expect decryptOutput.Failure?;
+
+        // Test Hierarchical Failures
+        decryptOutput := esdk.Decrypt(Types.DecryptInput(
+            ciphertext := esdkCiphertext,
+            materialsManager := None,
+            keyring := Some(hKeyring),
+            encryptionContext := None
+        ));
+
+        expect decryptOutput.Failure?;
+    }
+
+    method {:test} TestRemoveECAndSupplyMismatchedReprECFailure()
+    {
+
+        // encrypt remove(a) RSA {a, b} => decrypt {b:c} => fail
+        // encrypt remove(a) KMS {a, b} => decrypt {b:c} => fail
+        // encrypt remove(a) AES {a, b} => decrypt {b:c} => fail
+        // encrypt remove(a) Hie {a, b} => decrypt {b:c} => fail
+        
+        // The string "asdf" as bytes
+        var asdf := [ 97, 115, 100, 102 ];
+        
+        var defaultConfig := EncryptionSdk.DefaultAwsEncryptionSdkConfig();
+        var esdk :- expect EncryptionSdk.ESDK(config := defaultConfig);
+        var mpl :- expect MaterialProviders.MaterialProviders();
+
+        // get keyrings
+        var rsaKeyring := GetRsaKeyring();
+        var kmsKeyring := GetKmsKeyring();
+        var aesKeyring := GetAesKeyring();
+        var hKeyring := GetHierarchicalKeyring();
+        
+        var multiKeyring :- expect mpl.CreateMultiKeyring(mplTypes.CreateMultiKeyringInput(
+                                                            generator := Some(aesKeyring),
+                                                            childKeyrings := [rsaKeyring, kmsKeyring, hKeyring]
+                                                        ));
+
+        // FAILURE CASE 3
+        // Encrypt will not store all Encryption Context, we will drop one entry but it will still get included in the 
+        // header signture.
+        // Decrypt will supply the correct key but incorrect value; this MUST fail.
+        var encryptionContext := Fixtures.SmallEncryptionContext(Fixtures.SmallEncryptionContextVariation.AB);
+        var requiredECKeys := Fixtures.SmallEncryptionContextKeys(Fixtures.SmallEncryptionContextVariation.A);
+        // this reproduced encryption context contains the key we didn't store, but it has the wrong value
+        var mismatchedReproducedEncryptionContext := Fixtures.SmallMismatchedEncryptionContex(Fixtures.SmallEncryptionContextVariation.A); 
+        
+        var defaultCMM :- expect mpl.CreateDefaultCryptographicMaterialsManager(
+            mplTypes.CreateDefaultCryptographicMaterialsManagerInput(
+                keyring := multiKeyring
+            )
+        );
+
+        // Create Required EC CMM with the required EC Keys we want
+        var reqCMM :- expect mpl.CreateRequiredEncryptionContextCMM(
+            mplTypes.CreateRequiredEncryptionContextCMMInput(
+                underlyingCMM := Some(defaultCMM),
+                // At the moment reqCMM can only be created with a CMM, you cannot 
+                // create one by only passing in a keyring.
+                keyring := None,
+                requiredEncryptionContextKeys := requiredECKeys
+            )
+        );
+
+        var encryptOutput := esdk.Encrypt(Types.EncryptInput(
+            plaintext := asdf,
+            encryptionContext := Some(encryptionContext), 
+            materialsManager := Some(reqCMM),
+            keyring := None,
+            algorithmSuiteId := None,
+            frameLength := None
+        ));
+        
+        expect encryptOutput.Success?;
+        var esdkCiphertext := encryptOutput.value.ciphertext;
+        
+        // Test RSA Failure
+        var decryptOutput := esdk.Decrypt(Types.DecryptInput(
+            ciphertext := esdkCiphertext,
+            materialsManager := None,
+            keyring := Some(rsaKeyring),
+            encryptionContext := Some(mismatchedReproducedEncryptionContext)
+        ));
+        
+        expect decryptOutput.Failure?;
+
+        // Test KMS Failures
+        decryptOutput := esdk.Decrypt(Types.DecryptInput(
+            ciphertext := esdkCiphertext,
+            materialsManager := None,
+            keyring := Some(kmsKeyring),
+            encryptionContext := Some(mismatchedReproducedEncryptionContext)
+        ));
+        
+        expect decryptOutput.Failure?;
+
+        // Test AES Failures
+        decryptOutput := esdk.Decrypt(Types.DecryptInput(
+            ciphertext := esdkCiphertext,
+            materialsManager := None,
+            keyring := Some(aesKeyring),
+            encryptionContext := Some(mismatchedReproducedEncryptionContext)
+        ));
+        
+        expect decryptOutput.Failure?;
+
+        // Test Hierarchical Failures
+        decryptOutput := esdk.Decrypt(Types.DecryptInput(
+            ciphertext := esdkCiphertext,
+            materialsManager := None,
+            keyring := Some(hKeyring),
+            encryptionContext := Some(mismatchedReproducedEncryptionContext)
+        ));
+
+        expect decryptOutput.Failure?;
+    }
+
+    method {:test} TestRemoveECAndSupplyWithMissingRequiredValueDecryptFailure()
+    {
+        // encrypt remove(a) RSA {a, b} => decrypt remove(a) => fail
+        // encrypt remove(a) KMS {a, b} => decrypt remove(a) => fail
+        // encrypt remove(a) AES {a, b} => decrypt remove(a) => fail
+        // encrypt remove(a) Hie {a, b} => decrypt remove(a) => fail
+
+        // The string "asdf" as bytes
+        var asdf := [ 97, 115, 100, 102 ];
+        
+        var defaultConfig := EncryptionSdk.DefaultAwsEncryptionSdkConfig();
+        var esdk :- expect EncryptionSdk.ESDK(config := defaultConfig);
+        var mpl :- expect MaterialProviders.MaterialProviders();
+
+        // get keyrings
+        var rsaKeyring := GetRsaKeyring();
+        var kmsKeyring := GetKmsKeyring();
+        var aesKeyring := GetAesKeyring();
+        var hKeyring := GetHierarchicalKeyring();
+        
+        var multiKeyring :- expect mpl.CreateMultiKeyring(mplTypes.CreateMultiKeyringInput(
+                                                            generator := Some(aesKeyring),
+                                                            childKeyrings := [rsaKeyring, kmsKeyring, hKeyring]
+                                                        ));
+
+        // FAILURE CASE 4
+        // Encrypt will not store all Encryption Context, we will drop one entry but it will still get included in the 
+        // header signture.
+        // Decrypt will supply the correct key but incorrect value; this MUST fail.
+        var encryptionContext := Fixtures.SmallEncryptionContext(Fixtures.SmallEncryptionContextVariation.AB);
+        var requiredECKeys := Fixtures.SmallEncryptionContextKeys(Fixtures.SmallEncryptionContextVariation.A);
+        // this reproduced encryption context does not contain the key that was dropped
+        var droppedRequiredKeyEncryptionContext := Fixtures.SmallEncryptionContext(Fixtures.SmallEncryptionContextVariation.B); 
+        
+        var defaultCMM :- expect mpl.CreateDefaultCryptographicMaterialsManager(
+            mplTypes.CreateDefaultCryptographicMaterialsManagerInput(
+                keyring := multiKeyring
+            )
+        );
+
+        // Create Required EC CMM with the required EC Keys we want
+        var reqCMM :- expect mpl.CreateRequiredEncryptionContextCMM(
+            mplTypes.CreateRequiredEncryptionContextCMMInput(
+                underlyingCMM := Some(defaultCMM),
+                // At the moment reqCMM can only be created with a CMM, you cannot 
+                // create one by only passing in a keyring.
+                keyring := None,
+                requiredEncryptionContextKeys := requiredECKeys
+            )
+        );
+
+        var encryptOutput := esdk.Encrypt(Types.EncryptInput(
+            plaintext := asdf,
+            encryptionContext := Some(encryptionContext), 
+            materialsManager := Some(reqCMM),
+            keyring := None,
+            algorithmSuiteId := None,
+            frameLength := None
+        ));
+        
+        expect encryptOutput.Success?;
+        var esdkCiphertext := encryptOutput.value.ciphertext;
+        
+        // Test RSA Failure
+        var decryptOutput := esdk.Decrypt(Types.DecryptInput(
+            ciphertext := esdkCiphertext,
+            materialsManager := None,
+            keyring := Some(rsaKeyring),
+            encryptionContext := Some(droppedRequiredKeyEncryptionContext)
+        ));
+        
+        expect decryptOutput.Failure?;
+
+        // Test KMS Failure
+        decryptOutput := esdk.Decrypt(Types.DecryptInput(
+            ciphertext := esdkCiphertext,
+            materialsManager := None,
+            keyring := Some(kmsKeyring),
+            encryptionContext := Some(droppedRequiredKeyEncryptionContext)
+        ));
+        
+        expect decryptOutput.Failure?;
+
+        // Test AES Failure
+        decryptOutput := esdk.Decrypt(Types.DecryptInput(
+            ciphertext := esdkCiphertext,
+            materialsManager := None,
+            keyring := Some(aesKeyring),
+            encryptionContext := Some(droppedRequiredKeyEncryptionContext)
+        ));
+        
+        expect decryptOutput.Failure?;
+
+        // Test Hierarchical Failure
+        decryptOutput := esdk.Decrypt(Types.DecryptInput(
+            ciphertext := esdkCiphertext,
+            materialsManager := None,
+            keyring := Some(hKeyring),
+            encryptionContext := Some(droppedRequiredKeyEncryptionContext)
+        ));
+
+        expect decryptOutput.Failure?;
+
+    }
+
+    method {:test} TestReservedEncryptionContextKeyFailure()
+    {
+        // The string "asdf" as bytes
+        var asdf := [ 97, 115, 100, 102 ];
+        
+        var defaultConfig := EncryptionSdk.DefaultAwsEncryptionSdkConfig();
+        var esdk :- expect EncryptionSdk.ESDK(config := defaultConfig);
+        var mpl :- expect MaterialProviders.MaterialProviders();
+
+        // get keyrings
+        var rsaKeyring := GetRsaKeyring();
+        
+        var encryptionContext := Fixtures.GetResrvedECMap(); 
+        var requiredECKeys := [Fixtures.RESERVED_ENCRYPTION_CONTEXT];
+        
+        var defaultCMM :- expect mpl.CreateDefaultCryptographicMaterialsManager(
+            mplTypes.CreateDefaultCryptographicMaterialsManagerInput(
+                keyring := rsaKeyring
+            )
+        );
+
+        // Create Required EC CMM with the required EC Keys we want
+        // Although we are requesting that we remove a RESERVED key word from the encryption context
+        // The CMM instantiation will still succeed because the CMM is meant to work with different higher level
+        // encryption libraries who may have different reserved keys. Encryption will ultimately fail.
+        var reqCMM :- expect mpl.CreateRequiredEncryptionContextCMM(
+            mplTypes.CreateRequiredEncryptionContextCMMInput(
+                underlyingCMM := Some(defaultCMM),
+                // At the moment reqCMM can only be created with a CMM, you cannot 
+                // create one by only passing in a keyring.
+                keyring := None,
+                requiredEncryptionContextKeys := requiredECKeys
+            )
+        );
+        
+        var encryptOutput := esdk.Encrypt(Types.EncryptInput(
+            plaintext := asdf,
+            encryptionContext := Some(encryptionContext), 
+            materialsManager := Some(reqCMM),
+            keyring := None,
+            algorithmSuiteId := None,
+            frameLength := None
+        ));
+        
+        expect encryptOutput.Failure?;
+
+    }
+    
+    method GetHierarchicalKeyring() 
+        returns (output: mplTypes.IKeyring)
+        ensures output.ValidState() && fresh(output) && fresh(output.History) && fresh(output.Modifies)
+    {
+        var branchKeyId := BRANCH_KEY_ID;
+        var ttl : mplTypes.PositiveLong := (1 * 60000) * 10;
+        var mpl :- expect MaterialProviders.MaterialProviders();
+
+        var kmsClient :- expect KMS.KMSClient();
+        var ddbClient :- expect DDB.DynamoDBClient();
+        var kmsConfig := KeyStoreTypes.KMSConfiguration.kmsKeyArn(hierarchyKeyArn);
+
+        var keyStoreConfig := KeyStoreTypes.KeyStoreConfig(
+        id := None,
+        kmsConfiguration := kmsConfig,
+        logicalKeyStoreName := logicalKeyStoreName,
+        grantTokens := None,
+        ddbTableName := branchKeyStoreName,
+        ddbClient := Some(ddbClient),
+        kmsClient := Some(kmsClient)
+        );
+
+        var keyStore :- expect KeyStore.KeyStore(keyStoreConfig);
+
+        output :- expect mpl.CreateAwsKmsHierarchicalKeyring(
+            mplTypes.CreateAwsKmsHierarchicalKeyringInput(
+                branchKeyId := Some(branchKeyId),
+                branchKeyIdSupplier := None,
+                keyStore := keyStore,
+                ttlSeconds := ttl,
+                cache := None
+            ));
+    }
+
+    method GetRsaKeyring() 
+        returns (output: mplTypes.IKeyring)
+        ensures output.ValidState() && fresh(output) && fresh(output.History) && fresh(output.Modifies)
+    {
+        var mpl :- expect MaterialProviders.MaterialProviders();
+
+        var namespace, name := Fixtures.NamespaceAndName(0);
+        var keys := Fixtures.GenerateKeyPair(2048 as primitivesTypes.RSAModulusLengthBits);
+        output :- expect mpl.CreateRawRsaKeyring(mplTypes.CreateRawRsaKeyringInput(
+                                                            keyNamespace := namespace,
+                                                            keyName := name,
+                                                            paddingScheme := mplTypes.PaddingScheme.OAEP_SHA1_MGF1,
+                                                            publicKey := Option.Some(keys.publicKey.pem),
+                                                            privateKey := Option.Some(keys.privateKey.pem)
+                                                            ));
+        
+    }
+
+    method GetAesKeyring() 
+        returns (output: mplTypes.IKeyring)
+        ensures output.ValidState() && fresh(output) && fresh(output.History) && fresh(output.Modifies)
+    {
+        var mpl :- expect MaterialProviders.MaterialProviders();
+
+        var namespace, name := Fixtures.NamespaceAndName(0);
+        output :- expect mpl.CreateRawAesKeyring(mplTypes.CreateRawAesKeyringInput(
+                                                            keyNamespace := namespace,
+                                                            keyName := name,
+                                                            wrappingKey := seq(32, i => 0),
+                                                            wrappingAlg := mplTypes.ALG_AES256_GCM_IV12_TAG16
+                                                            ));
+    }
+
+    method GetKmsKeyring() 
+        returns (output: mplTypes.IKeyring)
+        ensures output.ValidState() && fresh(output) && fresh(output.History) && fresh(output.Modifies)
+    {
+        var kmsKey :=  Fixtures.keyArn;
+        var defaultConfig := EncryptionSdk.DefaultAwsEncryptionSdkConfig();
+        var esdk :- expect EncryptionSdk.ESDK(config := defaultConfig);
+        var mpl :- expect MaterialProviders.MaterialProviders();
+        var clientSupplier :- expect mpl.CreateDefaultClientSupplier(mplTypes.CreateDefaultClientSupplierInput);
+        var kmsClient :- expect clientSupplier.GetClient(mplTypes.GetClientInput(region := "us-west-2"));
+        
+        output :- expect mpl.CreateAwsKmsKeyring(
+            mplTypes.CreateAwsKmsKeyringInput(
+                kmsKeyId := kmsKey,
+                kmsClient := kmsClient,
+                grantTokens := None
+            )
+        );
+
+    }
+    
+} 
